progs/list_dt.v
@@ -15,6 +15,395 @@ Class listspec (list_struct: type) (list_link: ident) :=
 Section LIST.
 Context  {list_struct: type} {list_link: ident}.
 
+Definition links' (ls: listspec list_struct list_link) (sh: share) := 
+  HORec (fun (R: (list val)*(val*val) -> mpred) (lp: (list val)*(val*val)) =>
+        match lp with
+        | (h::hs, (first,last)) =>
+                (!! (h=first /\ ~ (ptr_eq first last)) && 
+                        EX tail:val, 
+                           field_mapsto sh list_struct list_link first tail
+                           * |> R (hs, (tail, last)))
+        | (nil, (first,last)) =>
+                 !! (ptr_eq first last) && emp
+        end).
+
+Definition links (ls: listspec list_struct list_link) (sh: share) (contents: list val) (x y: val) : mpred :=
+  links' ls sh (contents,(x,y)).
+
+Lemma links_unfold (ls: listspec list_struct list_link): forall sh contents v1 v2,
+  links ls sh contents v1 v2 = 
+  match contents with
+  | h::t => !!(h=v1 /\ ~ptr_eq v1 v2) && EX tail: val, 
+                           field_mapsto sh list_struct list_link v1 tail
+                           * |> links ls sh t tail v2
+  | nil => !! (ptr_eq v1 v2) && emp
+ end.
+Proof.
+ intros. unfold links.
+ unfold links' at 1. rewrite HORec_fold_unfold; auto.
+ apply prove_HOcontractive; intros.
+ destruct x. destruct l. 
+ auto 50 with contractive.
+ destruct p.
+ auto 50 with contractive.
+Qed.
+
+Lemma links_eq (ls: listspec list_struct list_link):
+  forall sh l v , 
+  typecheck_val v (tptr list_struct) = true ->
+    links ls sh l v v = !!(l=nil) && emp.
+Proof.
+intros.
+rewrite (links_unfold ls sh l v v).
+destruct l.
+f_equal. f_equal.
+unfold ptr_eq.
+unfold typecheck_val in H.
+destruct v; simpl in H; try discriminate; unfold Int.cmpu; rewrite Int.eq_true.
+apply prop_ext; intuition.
+apply prop_ext; intuition.
+apply pred_ext; normalize.
+contradiction H0.
+unfold ptr_eq, typecheck_val in H|-*.
+destruct v0; inv H; auto.
+unfold Int.cmpu.
+rewrite Int.eq_true. auto.
+unfold Int.cmpu.
+rewrite Int.eq_true. auto.
+inv H0.
+Qed.
+
+Definition links_cons (ls: listspec list_struct list_link) sh (l: list val) (x z: val) : mpred :=
+        !! (~ ptr_eq x z) && 
+       EX r:list val, EX y:val, 
+             !!(l=x::r  /\ typecheck_val y (tptr list_struct) = true) && 
+             field_mapsto sh list_struct list_link x y * 
+             |> links ls sh r y z.
+
+Lemma links_neq (ls: listspec list_struct list_link):  forall sh l x z , 
+  typecheck_val x (tptr list_struct) = true ->
+  typecheck_val z (tptr list_struct) = true ->
+  ptr_neq x z -> 
+    links ls sh l x z = links_cons ls sh l x z.
+Proof.
+unfold links_cons, ptr_neq; intros.
+rewrite links_unfold at 1; auto.
+destruct l.
+apply pred_ext; apply derives_extract_prop; intro.
+contradiction. clear H2.
+apply exp_left; intro r.
+apply exp_left; intro y.
+repeat rewrite sepcon_andp_prop'; apply derives_extract_prop; intros [? ?].
+inv H2.
+apply pred_ext; apply derives_extract_prop; intro.
+destruct H2 as [? _]. subst x.
+apply exp_left; intro tail.
+apply andp_right; try apply prop_right; auto.
+apply exp_right with l.
+apply exp_right with tail.
+repeat rewrite sepcon_andp_prop'; apply andp_right.
+rewrite (field_mapsto_typecheck_val list_struct list_link sh v tail list_structid list_fields noattr)
+  by apply list_struct_eq.
+rewrite list_link_type.
+normalize. auto.
+apply exp_left; intro r'.
+apply exp_left; intro y.
+repeat rewrite sepcon_andp_prop'; apply derives_extract_prop; intros [? ?].
+inv H3.
+apply andp_right.
+apply prop_right; auto.
+apply exp_right with y.
+ auto.
+Qed.
+
+Lemma links_unroll (ls: listspec list_struct list_link): forall sh l x z , 
+    links ls sh l x z = (!! (ptr_eq x z) && !! (l=nil) && emp) || links_cons ls sh l x z.
+Proof.
+intros.
+rewrite links_unfold at 1.
+apply pred_ext; destruct l.
+normalize.
+apply orp_right1; auto.
+apply orp_right2.
+unfold links_cons.
+normalize.
+apply exp_right with l.
+normalize.
+apply exp_right with tail.
+normalize.
+apply andp_right.
+erewrite (field_mapsto_typecheck_val list_struct list_link sh v tail); try reflexivity.
+rewrite list_link_type.
+normalize.
+apply list_struct_eq.
+auto.
+apply orp_left; normalize.
+unfold links_cons.
+normalize. inv H0.
+apply orp_left.
+normalize. inv H0.
+unfold links_cons.
+normalize.
+intros. symmetry in H0; inv H0.
+apply exp_right with y.
+normalize.
+Qed.
+
+Lemma links_nonnull (ls: listspec list_struct list_link):
+  forall sh s v,
+      typed_true (tptr list_struct) v ->
+     links ls sh s v nullval = links_cons ls sh s v nullval.
+Proof.
+intros. subst. 
+rewrite links_unroll.
+apply pred_ext; normalize.
+apply orp_left; auto. normalize.
+unfold typed_true, strict_bool_val,ptr_eq in *.
+destruct v; simpl in *; try contradiction.
+rewrite H0 in H. inv H.
+apply orp_right2. auto.
+Qed.
+
+Lemma links_nil_eq (ls: listspec list_struct list_link): 
+    forall sh p q, links ls sh nil p q = !! (ptr_eq p q) && emp.
+Proof. intros.
+ rewrite links_unroll.
+ apply pred_ext.
+ apply orp_left. normalize.
+ normalize. unfold links_cons. normalize. inv H0.
+ apply orp_right1. normalize.
+Qed.
+
+Lemma links_cons_eq (ls: listspec list_struct list_link):
+     forall sh h r x z , 
+    links ls sh (h::r) x z = 
+        !!(h=x /\ ~ ptr_eq x z) &&
+         (EX  y : val,
+          !!(typecheck_val y (tptr list_struct) = true) &&
+   field_mapsto sh list_struct list_link x y *
+   |>links ls sh r y z).
+Proof.
+ intros. rewrite links_unroll.
+ apply pred_ext.
+ apply orp_left.
+ rewrite andp_assoc.
+ apply derives_extract_prop; intro.
+ apply derives_extract_prop; intro.
+ inv H0.
+ unfold links_cons.
+ normalize. inv H0. intros r0 ?.
+ apply exp_right with r0.
+ repeat apply andp_right; try apply prop_right; auto.
+ normalize.
+ normalize.
+ apply orp_right2.
+ unfold links_cons.
+ apply andp_right. apply prop_right; auto.
+ apply exp_right with r.
+ apply exp_right with y.
+ normalize.
+Qed.
+
+Lemma eqp_e {A} {NA: NatDed A}{IA: Indir A}{RA: RecIndir A}:
+  forall (P Q : A), (TT |-- P <=> Q) -> P=Q.
+Proof.
+intros.
+apply pred_ext;
+(apply subp_e; eapply derives_trans; [apply H | apply fash_derives]).
+apply andp_left1; auto.
+apply andp_left2; auto.
+Qed.
+
+Lemma eqp_i1 {A} {NA: NatDed A}{IA: Indir A}{RA: RecIndir A}:
+  forall P (Q R : A),
+     unfash P && Q |-- R ->
+     unfash P && R |-- Q ->
+    P |-- Q <=> R.
+Proof.
+ intros.
+ rewrite fash_andp; apply andp_right; apply subp_i1; auto.
+Qed.
+
+
+Lemma ptr_eq_dec:
+  forall x z, {ptr_eq x z}+{~ptr_eq x z}.
+Proof.
+unfold ptr_eq; intros.
+destruct x; simpl; auto. destruct z; simpl; auto. destruct (Int.eq i i0); auto.
+destruct z; auto. destruct (eq_dec b b0).
+subst. destruct (Int.eq i i0); auto. right; intros [? ?]; auto. inv H0.
+right; intros [? ?]. contradiction.
+Qed.
+
+
+Lemma list_last: forall {A} (l: list A),
+   l=nil \/ exists prefix, exists y, l = prefix ++ y :: nil.
+Proof.
+induction l.
+left; auto.
+right.
+destruct IHl as [? | [prefix [y ?]]].
+subst. exists nil, a; auto.
+subst. exists (a::prefix), y; auto.
+Qed.
+
+
+Lemma allp_andp1  {A}{ND: NatDed A}:  forall B (any: B) (p: B -> A) q, andp (allp p) q = (allp (fun x => andp (p x) q)).
+Proof.
+ intros. apply pred_ext.
+ apply allp_right; intro x.
+ apply andp_derives; auto. apply allp_left with x; auto.
+ apply andp_right. apply allp_right; intro x. apply allp_left with x. apply andp_left1; auto.
+ apply allp_left with any. apply andp_left2; auto.
+Qed.
+
+Lemma allp_andp2  {A}{ND: NatDed A}:  forall B (any: B) p (q: B -> A), 
+     andp p (allp q) = (allp (fun x => andp p (q x))).
+Proof.
+intros. rewrite andp_comm. rewrite allp_andp1; auto.
+f_equal. extensionality x. rewrite andp_comm; auto.
+Qed.
+
+
+Lemma links_cons_right_null (ls: listspec list_struct list_link): forall sh l x y, 
+             field_mapsto sh list_struct list_link y nullval * 
+             links ls sh l x y
+   |--   links ls sh (l++y::nil) x nullval.
+Proof.
+intros.
+assert (TT |-- ALL l: list val, ALL x: val,
+                   (field_mapsto sh list_struct list_link y nullval * links ls sh l x y)  
+                     >=> links ls sh (l++y::nil) x nullval).
+Focus 2.
+apply subp_e; eapply derives_trans; [apply H | apply allp_left with l; apply allp_left with x; auto].
+clear x l.
+apply loeb.
+apply allp_right; intro l.
+apply allp_right; intro x.
+destruct l.
+rewrite links_nil_eq.
+apply derives_trans with TT; auto.
+apply subp_i1.
+apply andp_left2.
+normalize.
+simpl.
+assert (x=y) by (apply ptr_eq_e; auto). subst y.
+rewrite field_mapsto_isptr.
+normalize.
+rewrite links_cons_eq.
+apply andp_right.  apply prop_right; auto.
+split; auto. intro. apply ptr_eq_e in H1. subst. apply H0.
+apply exp_right with nullval.
+normalize.
+rewrite links_nil_eq.
+normalize.
+apply derives_trans with (field_mapsto sh list_struct list_link x nullval * emp).
+rewrite sepcon_emp; auto.
+apply sepcon_derives; auto.
+apply now_later.
+apply subp_i1.
+simpl app.
+rewrite links_cons_eq.
+rewrite links_cons_eq.
+autorewrite with norm.
+apply exp_left; intro z.
+apply exp_right with z.
+repeat rewrite sepcon_andp_prop'.
+rewrite andp_comm. rewrite andp_assoc.
+rewrite sepcon_comm.
+repeat rewrite andp_assoc.
+repeat rewrite sepcon_andp_prop'.
+repeat rewrite andp_assoc.
+apply derives_extract_prop; intro.
+apply derives_extract_prop; intro.
+apply derives_extract_prop; intro.
+subst v.
+apply andp_right. apply prop_right; auto.
+rewrite field_mapsto_isptr.
+normalize.
+apply andp_right. apply prop_right; auto.
+intro. apply ptr_eq_e in H2. subst; apply H.
+apply andp_right. apply prop_right; auto.
+rewrite prop_true_andp by auto.
+rewrite sepcon_assoc.
+rewrite andp_comm.
+rewrite unfash_sepcon_distrib.
+apply sepcon_derives.
+apply andp_left2; auto.
+rewrite <- later_unfash.
+eapply derives_trans.
+apply andp_derives; [apply derives_refl | ].
+apply sepcon_derives; [apply derives_refl | apply now_later].
+rewrite <- later_sepcon. rewrite <- later_andp.
+apply later_derives.
+rewrite unfash_allp.
+rewrite allp_andp1 by apply nil. apply allp_left with l.
+rewrite unfash_allp. rewrite allp_andp1 by apply Vundef. apply allp_left with z.
+destruct l.
+simpl.
+rewrite links_nil_eq.
+apply andp_left2.
+normalize. apply ptr_eq_e in H2. subst z.
+rewrite links_cons_eq.
+rewrite field_mapsto_isptr.
+normalize.
+apply exp_right with nullval.
+apply andp_right.
+apply prop_right.
+intro. apply ptr_eq_e in H3. subst. apply H2.
+normalize.
+rewrite links_nil_eq. normalize.
+eapply derives_trans; [ | apply sepcon_derives; [ apply derives_refl | apply now_later]].
+rewrite sepcon_emp; auto.
+eapply derives_trans.
+apply andp_derives; [apply unfash_fash | apply derives_refl].
+rewrite andp_comm. 
+apply derives_trans
+ with ((field_mapsto sh list_struct list_link y nullval *  links ls sh (v::l) z y ) &&
+   (field_mapsto sh list_struct list_link y nullval *  links ls sh (v::l) z y 
+     --> links ls sh ((v::l) ++ y :: nil) z nullval)).
+2: apply modus_ponens.
+apply andp_derives; auto.
+rewrite sepcon_comm.
+auto.
+Qed.
+
+Lemma ptr_eq_refl: forall x, isptr x -> ptr_eq x x.
+Proof.
+destruct x; simpl; intros; try contradiction.
+split; auto. apply Int.eq_true.
+Qed.
+
+
+Lemma links_cons_right_null' (ls: listspec list_struct list_link): forall sh l x y, 
+     links ls sh (l++y::nil) x nullval
+    |-- links ls sh l x y * |> field_mapsto sh list_struct list_link y nullval.
+Proof.
+(* Not provable.  The subtle reason is:
+  If l<>nil, cannot prove that x<>y.
+  One can prove that later-later-later, x<>y, but not now x<>y.
+*)
+Abort.
+
+Lemma links_cons_right (ls: listspec list_struct list_link): forall sh l x y z w, 
+             field_mapsto sh list_struct list_link y z * 
+             field_mapsto sh list_struct list_link z w * 
+             links ls sh l x y
+   |--   links ls sh (l++y::nil) x z * field_mapsto sh list_struct list_link z w.
+Admitted.
+
+
+Lemma links_unroll_right (ls: listspec list_struct list_link): forall sh l x z , 
+    links ls sh l x z = 
+             (!! (ptr_eq x z) && !! (l=nil) && emp) 
+           || (!! (~ ptr_eq x z) && 
+                EX h:val, EX r:list val, EX y:val, 
+                    !!(l=r++h::nil)  && 
+             field_mapsto sh list_struct list_link y z * 
+             |> links ls sh r x y).
+Proof.
+Abort.  (* probably not true *)
+
 Fixpoint all_but_link (ls: listspec list_struct list_link) (f: fieldlist) : fieldlist :=
  match f with
  | Fnil => Fnil
@@ -175,17 +564,6 @@ intros. symmetry in H0; inv H0.
 apply exp_right with y.
 normalize.
 Qed.
-
-Lemma ptr_eq_dec:
-  forall x z, {ptr_eq x z}+{~ptr_eq x z}.
-Proof.
-unfold ptr_eq; intros.
-destruct x; simpl; auto. destruct z; simpl; auto. destruct (Int.eq i i0); auto.
-destruct z; auto. destruct (eq_dec b b0).
-subst. destruct (Int.eq i i0); auto. right; intros [? ?]; auto. inv H0.
-right; intros [? ?]. contradiction.
-Qed.
-
 
 Lemma lseg_unroll_nonempty1 (ls: listspec list_struct list_link):
    forall p P sh h tail v1 v2,
@@ -357,10 +735,109 @@ Definition lseg_cons_right (ls: listspec list_struct list_link) sh (l: list (ele
              field_mapsto sh list_struct list_link y z * 
              |> lseg ls sh r x y.
 
+Lemma lseg_cons_right_null (ls: listspec list_struct list_link): forall sh l x h y, 
+             list_cell ls sh y h * field_mapsto sh list_struct list_link y nullval * 
+             lseg ls sh l x y
+   |--   lseg ls sh (l++h::nil) x nullval.
+Proof.
+intros.
+assert (TT |-- ALL l: list (elemtype ls), ALL x: val,
+                   (list_cell ls sh y h * field_mapsto sh list_struct list_link y nullval * lseg ls sh l x y)  
+                     >=> lseg ls sh (l++h::nil) x nullval).
+Focus 2.
+apply subp_e; eapply derives_trans; [apply H | apply allp_left with l; apply allp_left with x; auto].
+clear x l.
+apply loeb.
+apply allp_right; intro l.
+apply allp_right; intro x.
+destruct l.
+rewrite lseg_nil_eq.
+apply derives_trans with TT; auto.
+apply subp_i1.
+apply andp_left2.
+normalize.
+simpl.
+assert (x=y) by (apply ptr_eq_e; auto). subst y.
+rewrite field_mapsto_isptr.
+normalize.
+rewrite lseg_cons_eq.
+apply andp_right.  apply prop_right; auto.
+intro. apply ptr_eq_e in H1. subst. apply H0.
+apply exp_right with nullval.
+normalize.
+rewrite lseg_nil_eq.
+normalize.
+cancel. apply now_later.
+apply subp_i1.
+simpl app.
+rewrite andp_comm.
+rewrite lseg_cons_eq.
+rewrite lseg_cons_eq.
+autorewrite with norm.
+apply exp_left; intro z.
+apply exp_right with z.
+repeat rewrite sepcon_andp_prop'.
+rewrite andp_assoc.
+rewrite sepcon_comm.
+repeat rewrite andp_assoc.
+repeat rewrite sepcon_andp_prop'.
+repeat rewrite andp_assoc.
+apply derives_extract_prop; intro.
+apply derives_extract_prop; intro.
+rewrite field_mapsto_isptr.
+normalize.
+apply andp_right. apply prop_right; auto.
+intro. apply ptr_eq_e in H2. subst; apply H1.
+apply andp_right. apply prop_right; auto.
+apply andp_right. apply prop_right; auto.
+forget (list_cell ls sh x e * field_mapsto sh list_struct list_link x z) as A.
+rewrite sepcon_assoc.
+rewrite andp_comm.
+rewrite unfash_sepcon_distrib.
+apply sepcon_derives.
+apply andp_left2; auto.
+rewrite <- later_unfash.
+eapply derives_trans.
+apply andp_derives; [apply derives_refl | ].
+apply sepcon_derives; [apply derives_refl | apply now_later].
+rewrite <- later_sepcon. rewrite <- later_andp.
+apply later_derives.
+rewrite unfash_allp.
+rewrite allp_andp1 by apply nil. apply allp_left with l.
+rewrite unfash_allp. rewrite allp_andp1 by apply Vundef. apply allp_left with z.
+destruct l.
+simpl.
+rewrite lseg_nil_eq.
+apply andp_left2.
+normalize. apply ptr_eq_e in H2. subst z.
+rewrite lseg_cons_eq.
+rewrite field_mapsto_isptr.
+normalize.
+apply exp_right with nullval.
+apply andp_right.
+apply prop_right.
+intro. apply ptr_eq_e in H3. subst. apply H2.
+normalize.
+rewrite lseg_nil_eq. normalize.
+eapply derives_trans; [ | apply sepcon_derives; [ apply derives_refl | apply now_later]].
+rewrite sepcon_emp; auto.
+eapply derives_trans.
+apply andp_derives; [apply unfash_fash | apply derives_refl].
+rewrite andp_comm. 
+apply derives_trans
+ with ((list_cell ls sh y h * field_mapsto sh list_struct list_link y nullval *  lseg ls sh (e0::l) z y ) &&
+   (list_cell ls sh y h * field_mapsto sh list_struct list_link y nullval *  lseg ls sh (e0::l) z y 
+     --> lseg ls sh ((e0::l) ++ h :: nil) z nullval)).
+2: apply modus_ponens.
+apply andp_derives; auto.
+rewrite sepcon_comm.
+auto.
+Qed.
+
 
 Lemma lseg_unroll_right (ls: listspec list_struct list_link): forall sh l x z , 
     lseg ls sh l x z = (!! (ptr_eq x z) && !! (l=nil) && emp) || lseg_cons_right ls sh l x z.
-Admitted.
+Abort.  (* not likely true *)
 
 End LIST.
 
